theories/FOL/Incompleteness/fol_incompleteness.v
@@ -4,8 +4,9 @@ From Undecidability.Shared Require Import Dec embed_nat.
 From Undecidability.FOL.Util Require Import Syntax_facts FullDeduction FullDeduction_facts FullTarski FullTarski_facts Axiomatisations FA_facts Syntax.
 From Undecidability.FOL Require Import PA.
 From Undecidability.FOL.Proofmode Require Import Theories ProofMode Hoas.
-From Undecidability.FOL.Incompleteness Require Import formal_systems abstract_incompleteness fol qdec repr utils churchs_thesis.
+From Undecidability.FOL.Incompleteness Require Import formal_systems abstract_incompleteness fol qdec repr utils churchs_thesis dprm.
 
+From Undecidability.H10 Require Import DPRM dio_single.
 
 From Equations Require Import Equations.
 Require Import String List.
@@ -55,225 +56,121 @@ Proof.
   - intros [k Hk]. eapply List.nth_error_In, Hk.
 Qed.
 
+
 Section fol.
   Existing Instance PA_funcs_signature.
   Existing Instance PA_preds_signature.
-  Hypothesis (p : peirce).
-  Existing Instance intu.
 
-  Variable T : theory.
-  Hypothesis T_Q : list_theory Qeq ⊑ T.
-  Hypothesis Tenum : enumerable T.
-  Hypothesis Tconsis : ~@tprv _ _ _ p T ⊥.
 
-  Variable theta : nat -> nat -\ bool.
-  Variable theta_univ : is_universal theta.
+  Section incomplete_strong_repr.
+    Hypothesis (p : peirce).
 
-  Hypothesis Hrepr : forall P : nat -> Prop, enumerable P ->
-    exists φ, Qdec φ /\ bounded 2 φ /\ forall x ρ, P x <-> interp_nat; ρ ⊨ ∃φ[(num x)..].
+    Variable theta : nat -> nat -\ bool.
+    Hypothesis theta_universal : is_universal theta.
 
-  Lemma fol_incomplete' : exists φ, ~@tprv _ _ _ p T φ /\ ~@tprv _ _ _ p T (¬φ).
-  Proof.
-    assert (Qenum : enumerable (list_theory Qeq)) by apply list_theory_enumerable.
-    assert (Qconsis : ~list_theory Qeq ⊢TI ⊥).
-    { intros H.
-      assert (H' : Qeq ⊢ ⊥).
-      { destruct H as (Qeq' & Hc & H).
-        eapply Weak.
-        - apply H.
-        - exact Hc. }
-      eapply Q_sound_intu with (rho := fun _ => 0) in H' as []. }
-    eapply insep_essential_incompleteness with (fs := fol_fs Tenum Tconsis) (fs' := @fol_fs intu (list_theory Qeq) Qenum Qconsis).
-    - eapply theta_univ.
-    - intros φ Hφ.
-      eapply WeakT. 2: apply T_Q.
-      cbn in Hφ.
-      destruct Hφ as [Qeq' [Hc H]].
-      exists Qeq'. split; first assumption.
-      admit.
-    - cbn.
-      destruct (@Hrepr (fun x => theta x x ▷ true)) as [φ1 (HQ1 & Hb1 & Hφ1)].
-      { admit. }
-      destruct (@Hrepr (fun x => theta x x ▷ false)) as [φ2 (HQ2 & Hb2 & Hφ2)].
-      { admit. }
-      destruct (@weak_strong (fun x => theta x x ▷ true) 
-        (fun x => theta x x ▷ false)) with (φ1 := φ1) (φ2 := φ2) as (φ & Hb & Hφ).
-      + intros x H1 H2. enough (true = false) by discriminate. eapply part_functional; eassumption.
-      + assumption.
-      + assumption.
-      + assumption.
-      + assumption.
-      + admit.
-      + admit.
-      + exists (fun x => φ[(num x)..]). intros c. split.
-        * intros H. exists Qeq. split; first auto. now apply Hφ.
-        * intros H. exists Qeq. split; first auto. now apply Hφ.
-  Admitted.
+    Variable T : theory.
+    Hypothesis Tenum : enumerable T.
+    Hypothesis Tconsis : ~T ⊢T ⊥.
+
+    Variable T' : theory.
+    Hypothesis T'_T : T' ⊑ T.
+    Hypothesis T'enum : enumerable T'.
+
+    Variable r : nat -> form.
+    Hypothesis Hrepr : forall c,
+      (theta c c ▷ true -> T' ⊢T r c) /\
+      (theta c c ▷ false -> T' ⊢T ¬r c).
+
+    Lemma fol_incomplete_strong_repr : exists n, ~T ⊢T r n /\ ~T ⊢T ¬r n.
+    Proof.
+      assert (~T' ⊢T ⊥) as T'consis.
+      { contradict Tconsis. now eapply WeakT. }
+      apply (insep_essential_incompleteness) with (theta := theta) (fs := fol_fs Tenum Tconsis) (fs' := fol_fs T'enum T'consis).
+      - assumption.
+      - unfold extension. cbn. intros φ Hφ. now eapply WeakT.
+      - assumption.
+    Qed.
+  End incomplete_strong_repr.
+
+
+
+
+  Section Q_weakly_represents.
+    Existing Instance intu.
+    Hypothesis mu_universal : mu_is_universal.
+
+    Variable P : nat -> Prop.
+    Hypothesis Penum : enumerable P. 
+    Lemma Q_weak_repr : exists φ, bounded 1 φ /\ Σ1 φ /\ forall x, P x <-> Qeq ⊢ φ[(num x)..].
+    Proof.
+      destruct mu_recursive_definable with (P := P) (peirc := intu) as (φ & Hb & HΣ & Hr).
+      { now apply mu_semi_decidable_enumerable. }
+      exists φ. do 2 (split; first assumption).
+      intros x. erewrite Hr. instantiate (1 := fun _ => 0). split.
+      - intros H. eapply Σ1_completeness.
+        + now apply Σ1_subst.
+        + eapply subst_bound; first eassumption.
+          intros [|n] Hn; last lia. apply num_bound.
+        + now rewrite <-sat_single_nat.
+      - intros H. rewrite sat_single_nat. eapply soundness; first eassumption.
+        apply nat_is_Q_model.
+    Qed.
+  End Q_weakly_represents.
+  Check weak_strong.
+
+
+
+
+  Section Q_incomplete.
+    Hypothesis mu_universal : mu_is_universal.
+
+    (* TODO *)
+    Hypothesis (p : peirce).
+    Existing Instance intu.
+
+    Variable T : theory.
+    Hypothesis T_Q : list_theory Qeq ⊑ T.
+    Hypothesis Tenum : enumerable T.
+    Hypothesis Tconsis : ~@tprv _ _ _ p T ⊥.
+
+    Lemma theta_c_c_enumerable (theta : nat -> nat -\ bool) b : enumerable (fun c => theta c c ▷ b).
+    Proof. 
+      apply semi_decidable_enumerable.
+      { exists (fun n => Some n). intros n. now exists n. }
+      exists (fun c k => match core (theta c c) k, b with
+                         | Some true, true => true
+                         | Some false, false => true
+                         | _, _ => false
+                         end).
+     intros c. split; intros [k Hk]; exists k.
+     - rewrite Hk. destruct b; congruence.
+     - destruct (core _ _) as [[]|], b; congruence.
+    Qed. 
+    Theorem Q_incomplete : exists φ, bounded 0 φ /\ Σ1 φ /\ ~@tprv _ _ _ p T φ /\ ~@tprv _ _ _ p T (¬φ).
+    Proof. 
+      assert (exists f : nat -> nat -\ bool, is_universal f) as [theta theta_universal].
+      { apply ct_nat_bool, CTmu, mu_universal. }
+
+      destruct (@Q_weak_repr mu_universal (fun c => theta c c ▷ true) (theta_c_c_enumerable theta true)) as (φ1 & Hb1 & HΣ1 & Hφ1).
+      destruct (@Q_weak_repr mu_universal (fun c => theta c c ▷ false) (theta_c_c_enumerable theta false)) as (φ2 & Hb2 & HΣ2 & Hφ2).
+      assert (forall c, theta c c ▷ true -> theta c c ▷ false -> False) as Hdisj.
+      { intros c Ht Hf. enough (true = false) by discriminate. eapply part_functional; eassumption. }
+      edestruct (weak_strong Hdisj Hb1 Hb2 HΣ1 HΣ2 Hφ1 Hφ2) as (ψ & Hb & HΣ & Hψ1 & Hψ2).
+      edestruct (@fol_incomplete_strong_repr p theta theta_universal T Tenum Tconsis (list_theory Qeq) T_Q (list_theory_enumerable Qeq)).
+      { instantiate (1 := fun c => ψ[(num c)..]). cbn. 
+        intros c. split.
+        - intros H. exists Qeq. split; first auto.
+          now apply prv_intu_class.
+        - intros H. exists Qeq. split; first auto.
+          now apply prv_intu_class. }
+      cbn in H. exists ψ[(num x)..]. 
+      repeat apply conj.
+      - eapply subst_bound; first eassumption. intros [|n] Hn; last lia. apply num_bound.
+      - now apply Σ1_subst.
+      - apply H.
+      - apply H.
+    Qed.
+  End Q_incomplete.
+
 End fol.
-Section fol.
-  Existing Instance PA_funcs_signature.
-  Existing Instance PA_preds_signature.
-  Hypothesis (p : peirce).
 
-  Variable T : theory.
-  Hypothesis T_Q : list_theory Qeq ⊑ T.
-  Hypothesis Tenum : enumerable T.
-  Hypothesis Tconsis : ~@tprv _ _ _ p T ⊥.
-
-  Variable theta : nat -> nat -\ bool.
-  Variable theta_univ : is_universal theta.
-
-  Hypothesis Hrepr : forall P : nat -> Prop, enumerable P ->
-    exists φ, @Σ1 intu φ /\ bounded 1 φ /\ forall x ρ, P x <-> interp_nat; (x .: ρ) ⊨ φ.
-
-  Lemma fol_incomplete : exists φ, ~@tprv _ _ _ p T φ /\ ~@tprv _ _ _ p T (¬φ).
-  Proof.
-    eapply fol_incomplete'; try eassumption.
-    intros P Penum. destruct (Hrepr Penum) as (ψ & HΣ & Hb & Hc).
-    destruct (Σ1_compression Hb HΣ) as (ψ' & HQ & Hb' & Hc').
-    exists ψ'[$1 .: $0 ..]. split; last split.
-    { now apply Qdec_subst. }
-    { eapply subst_bound; first eassumption. intros [|[|n]]; cbn; solve_bounds. }
-    intros x ρ.
-    apply Q_sound_intu with (rho := x .: ρ) in Hc'. cbn in Hc'.
-    rewrite (Hc x ρ). 
-    eassert (Hc'' : _ <-> _) by exact Hc'. rewrite Hc''. cbn.
-    apply utils_tac.exists_equiv. intros k.
-    rewrite !sat_single_nat, !subst_comp. 
-    assert (H : forall phi1 phi2, phi1 = phi2 -> interp_nat; ρ ⊨ phi1 <-> interp_nat; ρ ⊨ phi2) by (now intros ? ? ->); apply H.
-    eapply bounded_subst; first eassumption. 
-    intros [|[|[|n]]]; cbn; rewrite ?num_subst; repeat solve_bounds.
-  Qed.
-
-End fol.
-
-From Undecidability.H10 Require Import DPRM dio_single.
-Section dprm.
-  Existing Instance PA_funcs_signature.
-  Existing Instance PA_preds_signature.
-  Existing Instance interp_nat.
-
-  Variable P : nat -> Prop.
-  Context `{peirc : peirce}.
-
-  Fixpoint fin_to_n k (n : Fin.t k) : nat.
-  Proof.
-    destruct n.
-    - exact 0.
-    - exact (S (fin_to_n _ n0)).
-  Defined.
-  Lemma fin_to_n_bound k (n : Fin.t k) :
-    fin_to_n n <= k.
-  Proof.
-    induction n; cbn; lia.
-  Qed.
-  Fixpoint embed_poly n (p : dio_polynomial (Fin.t n) (Fin.t 1)) : term.
-  Proof.
-    destruct p.
-    - exact (num n0).
-    - exact $(fin_to_n t).
-    - exact $n.
-    - destruct d.
-      + exact (embed_poly _ p1 ⊕ embed_poly _ p2).
-      + exact (embed_poly _ p1 ⊗ embed_poly _ p2).
-  Defined.
-  Lemma embed_poly_bound n (p : dio_polynomial (Fin.t n) (Fin.t 1)) :
-    bounded_t (S n) (embed_poly p).
-  Proof.
-    induction p; cbn.
-    - apply num_bound.
-    - constructor. pose proof (fin_to_n_bound v). lia.
-    - solve_bounds.
-    - destruct d; now solve_bounds.
-  Qed.
-
-  Fixpoint vec_pos_default {X : Type} {n : nat} (v : Vector.t X n) (d : nat -> X) k : X
-    := match v with
-       | Vector.nil => d k
-       | Vector.cons _ x n' v' => match k with 
-                                  | 0 => x
-                                  | S k' => vec_pos_default v' d k'
-                                  end
-       end.
-  Lemma vec_pos_default_fin {X : Type} {n : nat} (v : Vector.t X n) (f : Fin.t n) (d : nat -> X) :
-    vec.vec_pos v f = vec_pos_default v d (fin_to_n f).
-  Proof.
-    induction f; depelim v; now cbn.
-  Qed.
-  Lemma vec_pos_default_default {X : Type} {n : nat} (v : Vector.t X n) (m : nat) (d : nat -> X) :
-    d m = vec_pos_default v d (m + n).
-  Proof.
-    induction v; cbn.
-    - f_equal. lia.
-    - now replace (m + S n) with (S m + n) by lia.
-  Qed.
-
-  Lemma embed_eval n (p : dio_polynomial (Fin.t n) (Fin.t 1)) : 
-    forall x ρ (v : Vector.t nat n), 
-      dp_eval (vec.vec_pos v) (fun _ => x) p = eval (vec_pos_default v (x .: ρ)) (embed_poly p).
-  Proof. 
-    intros x ρ. induction p; intros w; cbn.
-    - now rewrite nat_eval_num.
-    - apply vec_pos_default_fin.
-    - change n with (0 + n).
-      now rewrite <-vec_pos_default_default with (m := 0).
-    - destruct d; cbn; now rewrite IHp1, IHp2.
-  Qed.
-
-  Lemma vec_pos_default_append n m (v : Vector.t nat n) (w : Vector.t nat m) d k :
-    vec_pos_default (Vector.append v w) d k = vec_pos_default v (vec_pos_default w d) k.
-  Proof.
-    induction v in k |-*; first reflexivity.
-    cbn. now destruct k.
-  Qed.
-  Lemma vec_append1 n (v : Vector.t nat (n+1)) :
-    exists k w, v = Vector.append w (Vector.cons k Vector.nil).
-  Proof.
-    induction n as [|n IHn].
-    - do 2 depelim v. now exists h, Vector.nil.
-    - cbn in v. depelim v. destruct (IHn v) as (k & w & ->). 
-      now exists k, (Vector.cons h w). 
-  Qed.
-
-  Lemma sat_exist_times n ρ φ : interp_nat; ρ ⊨ exist_times n φ <-> exists w : Vector.t nat n, interp_nat; (vec_pos_default w ρ) ⊨ φ.
-  Proof.
-    induction n as [|n IHn] in ρ |-*; cbn.
-    - split.
-      + intros H. now exists Vector.nil.
-      + intros [v H]. now depelim v. 
-    - setoid_rewrite IHn. split. 
-      + intros (k & w & Hw). replace (S n) with (n + 1) by lia.
-        exists (Vector.append w (Vector.cons k Vector.nil)).
-        eapply sat_ext; first apply vec_pos_default_append.
-        assumption.
-      + replace (S n) with (n+1) by lia.
-        intros [w Hw]. 
-        destruct (vec_append1 w) as (h & w' & ->).
-        exists h, w'.
-        eapply sat_ext in Hw.
-        2: { intros x. symmetry. apply vec_pos_default_append. }
-        easy.
-  Qed.
-
-  Lemma dprm_definable : dio_rec_single P -> exists φ, Σ1 φ /\ bounded 1 φ /\ forall x ρ, P x <-> interp_nat; (x .: ρ) ⊨ φ.
-  Proof.
-    unfold dio_rec_single.
-    intros (n & p1 & p2 & H).
-    exists (exist_times n (embed_poly p1 == embed_poly p2)). repeat apply conj.
-    - apply exist_times_Σ1. constructor. apply Qdec_eq.
-    - apply bounded_exist_times. 
-      all: replace (n + 1) with (S n) by lia.
-      solve_bounds; apply embed_poly_bound.
-    - intros x ρ. rewrite H. clear H. 
-      setoid_rewrite sat_exist_times. 
-      setoid_rewrite embed_eval. cbn. reflexivity.
-  Qed.
-
-  Check mu_recursive.
-  Lemma mu_recursive_definable : mu_recursive P -> exists φ, Σ1 φ /\ bounded 1 φ /\ forall x ρ, P x <-> interp_nat; (x .: ρ) ⊨ φ.
-  Proof.
-    intros H. apply dprm_definable. now do 3 apply DPRM_1.
-  Qed.
-  
-
-End dprm.
