theories/FOL/Incompleteness/dprm.v
@@ -1,0 +1,252 @@
+
+From Undecidability.Synthetic Require Import DecidabilityFacts EnumerabilityFacts ReducibilityFacts.
+
+From Undecidability.H10 Require Import DPRM dio_single.
+
+From Equations Require Import Equations.
+Require Import String List.
+From Undecidability.L.Reductions Require Import MuRec.
+From Undecidability.MuRec Require Import recalg.
+Require Import Undecidability.L.Reductions.MuRec.MuRec_extract.
+From Undecidability.H10 Require Import DPRM.
+Require Import Undecidability.Synthetic.EnumerabilityFacts.
+From Coq.Logic Require Import ConstructiveEpsilon.
+Require Import Equations.Equations.
+Import ListNotations.
+
+
+From Undecidability.FOL.Incompleteness Require Import utils churchs_thesis ra.
+
+Definition mu_semi_decidable (P : nat -> Prop) := 
+  exists f : recalg 1, forall x : nat,
+    P x <-> (exists y, ra_rel f (Vector.cons nat x 0 (Vector.nil nat)) y).
+
+Section recalg_enum.
+  Variable f : nat -> option (recalg 1).
+  Hypothesis f_enum : enumerator__T f (recalg 1).
+
+  Local Definition nat_recalg : nat -> option (recalg 1) := f.
+  Local Definition recalg_nat : recalg 1 -> nat.
+  Proof using f_enum.
+    intros c. destruct (constructive_indefinite_ground_description_nat_Acc (fun n => f n = Some c)) as [y _].
+    - intros n. decide equality. apply recalg_dec.
+    - apply f_enum.
+    - exact y.
+  Defined.
+  Local Lemma nat_recalg_nat r : nat_recalg (recalg_nat r) = Some r.
+  Proof. 
+    unfold nat_recalg, recalg_nat. now destruct constructive_indefinite_ground_description_nat_Acc.
+  Qed.
+End recalg_enum.
+Lemma recalg_invert : exists (f : recalg 1 -> nat) (g : nat -> option (recalg 1)), forall r, g (f r) = Some r.
+Proof.
+  destruct (enumT_recalg 1) as [enum Henum].
+  do 2 eexists. apply nat_recalg_nat.
+Qed.
+
+
+Lemma erase_ra_rel alg x y :
+  (exists k, evalfun k (erase alg) [x] = Some y) <-> 
+  ra_rel alg (Vector.cons _ x _ (Vector.nil _)) y.
+Proof.
+  split.
+  - intros [k Hk]. 
+    apply ra_bs_c_correct. exists k.
+    apply erase_correct. unfold evalfun in Hk.
+    cbn. now destruct eval as [[]|].
+  - intros H. apply ra_bs_c_correct in H as [k Hk].
+    exists k. apply erase_correct in Hk. cbn in Hk.
+    unfold evalfun. now destruct eval as [[]|].
+Qed.
+
+Import ListNotations.
+Definition mu_step : recalg 1 -> nat -\ nat.
+Proof.
+  intros c x. unshelve eexists.
+  { intros k. exact (evalfun k (erase c) [x]). }
+  unfold core_valid.
+  intros y1 y2 k1 k2 H1 H2. unfold evalfun in *.
+  eapply ra_rel_fun.
+  - apply erase_ra_rel. exists k1. eassumption.
+  - apply erase_ra_rel. exists k2. eassumption.
+Defined.
+Definition mu_is_universal := forall f, exists c, forall x y, f x ▷ y <-> mu_step c x ▷ y.
+Section mu.
+  Hypothesis mu_universal : mu_is_universal.
+
+  Lemma mu_semi_decidable_enumerable (P : nat -> Prop) :
+    enumerable P -> mu_semi_decidable P.
+  Proof using mu_universal.
+    intros [f Hf]%enumerable_semi_decidable; last apply discrete_nat.
+
+    unfold mu_semi_decidable. unfold semi_decider in Hf.
+
+    unshelve edestruct mu_universal as [c Hc].
+    { intros x. unshelve eexists.
+      { exact (fun k => if f x k then Some 0 else None). }
+      intros y1 y2 k1 k2 H1 H2.
+      destruct (f x k1) eqn:Hf1, (f x k2) eqn:Hf2; congruence. }
+    cbn in Hc.
+    exists c. intros x. rewrite Hf. split.
+    - intros [k Hk]. exists 0.
+      apply erase_ra_rel.
+      destruct (Hc x 0) as [[k' Hk'] _].
+      { exists k. cbn. now rewrite Hk. }
+      exists k'. assumption.
+    - intros [k Hk]. 
+      unfold "▷" in Hc. cbn in Hc.
+      apply erase_ra_rel, Hc in Hk as [k' Hk'].
+      exists k'. now destruct f.
+  Qed.
+
+  Lemma CTmu : exists f : nat -> nat -\ nat, is_universal f.
+  Proof using mu_universal.
+    destruct recalg_invert as (f & g & H). 
+    unshelve eexists.
+    { intros c. destruct (g c).
+      - apply (mu_step r).
+      - intros x. exists (fun _ => None). congruence. }
+    intros h. destruct (mu_universal h) as [r Hr].
+    exists (f r). now rewrite H.
+  Qed.
+
+End mu.
+
+
+From Undecidability.FOL.Util Require Import Syntax_facts FullDeduction FullDeduction_facts FullTarski FullTarski_facts Axiomatisations FA_facts Syntax.
+From Undecidability.FOL Require Import PA.
+
+From Undecidability.FOL.Incompleteness Require Import fol qdec.
+
+
+Section fol.
+  Existing Instance PA_funcs_signature.
+  Existing Instance PA_preds_signature.
+
+
+  Section dprm.
+    Existing Instance interp_nat.
+
+    Variable P : nat -> Prop.
+    Context `{peirc : peirce}.
+
+    Fixpoint fin_to_n k (n : Fin.t k) : nat.
+    Proof.
+      destruct n.
+      - exact 0.
+      - exact (S (fin_to_n _ n0)).
+    Defined.
+    Lemma fin_to_n_bound k (n : Fin.t k) :
+      fin_to_n n <= k.
+    Proof.
+      induction n; cbn; lia.
+    Qed.
+    Fixpoint embed_poly n (p : dio_polynomial (Fin.t n) (Fin.t 1)) : term.
+    Proof.
+      destruct p.
+      - exact (num n0).
+      - exact $(fin_to_n t).
+      - exact $n.
+      - destruct d.
+        + exact (embed_poly _ p1 ⊕ embed_poly _ p2).
+        + exact (embed_poly _ p1 ⊗ embed_poly _ p2).
+    Defined.
+    Lemma embed_poly_bound n (p : dio_polynomial (Fin.t n) (Fin.t 1)) :
+      bounded_t (S n) (embed_poly p).
+    Proof.
+      induction p; cbn.
+      - apply num_bound.
+      - constructor. pose proof (fin_to_n_bound v). lia.
+      - solve_bounds.
+      - destruct d; now solve_bounds.
+    Qed.
+
+    Fixpoint vec_pos_default {X : Type} {n : nat} (v : Vector.t X n) (d : nat -> X) k : X
+      := match v with
+         | Vector.nil => d k
+         | Vector.cons x n' v' => match k with 
+                                    | 0 => x
+                                    | S k' => vec_pos_default v' d k'
+                                    end
+         end.
+    Lemma vec_pos_default_fin {X : Type} {n : nat} (v : Vector.t X n) (f : Fin.t n) (d : nat -> X) :
+      vec.vec_pos v f = vec_pos_default v d (fin_to_n f).
+    Proof.
+      induction f; depelim v; now cbn.
+    Qed.
+    Lemma vec_pos_default_default {X : Type} {n : nat} (v : Vector.t X n) (m : nat) (d : nat -> X) :
+      d m = vec_pos_default v d (m + n).
+    Proof.
+      induction v; cbn.
+      - f_equal. lia.
+      - now replace (m + S n) with (S m + n) by lia.
+    Qed.
+
+    Lemma embed_eval n (p : dio_polynomial (Fin.t n) (Fin.t 1)) : 
+      forall x ρ (v : Vector.t nat n), 
+        dp_eval (vec.vec_pos v) (fun _ => x) p = eval (vec_pos_default v (x .: ρ)) (embed_poly p).
+    Proof. 
+      intros x ρ. induction p; intros w; cbn.
+      - now rewrite nat_eval_num.
+      - apply vec_pos_default_fin.
+      - change n with (0 + n).
+        now rewrite <-vec_pos_default_default with (m := 0).
+      - destruct d; cbn; now rewrite IHp1, IHp2.
+    Qed.
+
+    Lemma vec_pos_default_append n m (v : Vector.t nat n) (w : Vector.t nat m) d k :
+      vec_pos_default (Vector.append v w) d k = vec_pos_default v (vec_pos_default w d) k.
+    Proof.
+      induction v in k |-*; first reflexivity.
+      cbn. now destruct k.
+    Qed.
+    Lemma vec_append1 n (v : Vector.t nat (n+1)) :
+      exists k w, v = Vector.append w (Vector.cons k Vector.nil).
+    Proof.
+      induction n as [|n IHn].
+      - do 2 depelim v. now exists h, Vector.nil.
+      - cbn in v. depelim v. destruct (IHn v) as (k & w & ->). 
+        now exists k, (Vector.cons h w). 
+    Qed.
+
+    Lemma sat_exist_times n ρ φ : interp_nat; ρ ⊨ exist_times n φ <-> exists w : Vector.t nat n, interp_nat; (vec_pos_default w ρ) ⊨ φ.
+    Proof.
+      induction n as [|n IHn] in ρ |-*; cbn.
+      - split.
+        + intros H. now exists Vector.nil.
+        + intros [v H]. now depelim v. 
+      - setoid_rewrite IHn. split. 
+        + intros (k & w & Hw). replace (S n) with (n + 1) by lia.
+          exists (Vector.append w (Vector.cons k Vector.nil)).
+          eapply sat_ext; first apply vec_pos_default_append.
+          assumption.
+        + replace (S n) with (n+1) by lia.
+          intros [w Hw]. 
+          destruct (vec_append1 w) as (h & w' & ->).
+          exists h, w'.
+          eapply sat_ext in Hw.
+          2: { intros x. symmetry. apply vec_pos_default_append. }
+          easy.
+    Qed.
+
+    Lemma dprm_definable : dio_rec_single P -> exists φ, Σ1 φ /\ bounded 1 φ /\ forall x ρ, P x <-> interp_nat; (x .: ρ) ⊨ φ.
+    Proof.
+      unfold dio_rec_single.
+      intros (n & p1 & p2 & H).
+      exists (exist_times n (embed_poly p1 == embed_poly p2)). repeat apply conj.
+      - apply exist_times_Σ1. constructor. apply Qdec_eq.
+      - apply bounded_exist_times. 
+        all: replace (n + 1) with (S n) by lia.
+        solve_bounds; apply embed_poly_bound.
+      - intros x ρ. rewrite H. clear H. 
+        setoid_rewrite sat_exist_times. 
+        setoid_rewrite embed_eval. cbn. reflexivity.
+    Qed.
+
+    Lemma mu_recursive_definable : mu_semi_decidable P -> exists φ, Σ1 φ /\ bounded 1 φ /\ forall x ρ, P x <-> interp_nat; (x .: ρ) ⊨ φ.
+    Proof.
+      intros [r Hr]. apply dprm_definable. do 3 apply DPRM_1. now exists r.
+    Qed.
+    
+  End dprm.
+End fol.
