theories/FOL/Incompleteness/repr.v
@@ -44,173 +44,228 @@ Section value_disjoint.
   Existing Instance PA_preds_signature.
   Existing Instance intu.
 
-
   Variable P1 P2 : nat -> Prop.
   Hypothesis P_disjoint : forall x, P1 x -> P2 x -> False.
 
-  Variable φ1 φ2 : form.
-  Hypothesis (φ1_bounded : bounded 2 φ1) (φ2_bounded : bounded 2 φ2).
-  Hypothesis (φ1_qdec : Qdec φ1) (φ2_qdec : Qdec φ2).
-  Hypothesis (φ1_syn : forall x, P1 x <-> Qeq ⊢ ∃ φ1[(num x) ..])
-             (φ2_syn : forall x, P2 x <-> Qeq ⊢ ∃ φ2[(num x) ..]).
+  Section value_disjoint'.
+    Variable φ1 φ2 : form.
+    Hypothesis (φ1_bounded : bounded 2 φ1) (φ2_bounded : bounded 2 φ2).
+    Hypothesis (φ1_qdec : Qdec φ1) (φ2_qdec : Qdec φ2).
+    Hypothesis (φ1_syn : forall x, P1 x <-> Qeq ⊢ ∃ φ1[(num x) ..])
+               (φ2_syn : forall x, P2 x <-> Qeq ⊢ ∃ φ2[(num x) ..]).
 
-  Local Lemma φ1_sem x ρ : P1 x <-> interp_nat; ρ ⊨ ∃ φ1[(num x) ..].
-  Proof.
-    rewrite φ1_syn.
-    split.
-    - intros H%soundness. apply H, nat_is_Q_model.
-    - apply Σ1_completeness.
-      + do 2 constructor. now apply Qdec_subst.
-      + solve_bounds. eapply subst_bound; first eassumption.
-        intros [|[|n]] H; cbn. 2-3: solve_bounds.
-        apply num_bound.
-  Qed.
-  Local Lemma φ2_sem x ρ : P2 x <-> interp_nat; ρ ⊨ ∃ φ2[(num x) ..].
-  Proof.
-    rewrite φ2_syn.
-    split.
-    - intros H%soundness. apply H, nat_is_Q_model.
-    - apply Σ1_completeness.
-      + do 2 constructor. now apply Qdec_subst.
-      + solve_bounds. eapply subst_bound; first eassumption.
-        intros [|[|n]] H; cbn. 2-3: solve_bounds.
-        apply num_bound.
-  Qed.
-        
-  Definition φ1' := φ1 ∧ ∀ $0 ⧀= $2 ~> φ2[$1 .: $0 ..] ~> ⊥.
-  Definition φ2' := φ2 ∧ ∀ $0 ⧀= $2 ~> φ1[$1 .: $0 ..] ~> ⊥.
+    Local Lemma φ1_sem x ρ : P1 x <-> interp_nat; ρ ⊨ ∃ φ1[(num x) ..].
+    Proof.
+      rewrite φ1_syn.
+      split.
+      - intros H%soundness. apply H, nat_is_Q_model.
+      - apply Σ1_completeness.
+        + do 2 constructor. now apply Qdec_subst.
+        + solve_bounds. eapply subst_bound; first eassumption.
+          intros [|[|n]] H; cbn. 2-3: solve_bounds.
+          apply num_bound.
+    Qed.
+    Local Lemma φ2_sem x ρ : P2 x <-> interp_nat; ρ ⊨ ∃ φ2[(num x) ..].
+    Proof.
+      rewrite φ2_syn.
+      split.
+      - intros H%soundness. apply H, nat_is_Q_model.
+      - apply Σ1_completeness.
+        + do 2 constructor. now apply Qdec_subst.
+        + solve_bounds. eapply subst_bound; first eassumption.
+          intros [|[|n]] H; cbn. 2-3: solve_bounds.
+          apply num_bound.
+    Qed.
+          
+    Definition φ1' := φ1 ∧ ∀ $0 ⧀= $2 ~> φ2[$1 .: $0 ..] ~> ⊥.
+    Definition φ2' := φ2 ∧ ∀ $0 ⧀= $2 ~> φ1[$1 .: $0 ..] ~> ⊥.
 
-  Lemma φ1'_bounded : bounded 2 φ1'.
-  Proof.
-    unfold φ1'. rewrite pless_eq.
-    repeat solve_bounds.
-    - assumption.
-    - eapply subst_bound; first eassumption.
-      intros [|[|n]] H; cbn; solve_bounds.
-  Qed.
-  Lemma φ2'_bounded : bounded 2 φ2'.
-  Proof.
-    unfold φ2'. rewrite pless_eq.
-    repeat solve_bounds.
-    - assumption.
-    - eapply subst_bound; first eassumption.
-      intros [|[|n]] H; cbn; solve_bounds.
-  Qed.
-  Lemma φ1'_qdec : Qdec φ1'.
-  Proof.
-    apply Qdec_and; first assumption.
-    apply (@Qdec_bounded_forall _ 1).
-    apply Qdec_impl.
-    - apply Qdec_subst, φ2_qdec.
-    - apply Qdec_bot.
-  Qed.
-  Lemma φ2'_qdec : Qdec φ2'.
-  Proof.
-    apply Qdec_and; first assumption.
-    apply (@Qdec_bounded_forall _ 1).
-    apply Qdec_impl.
-    - apply Qdec_subst, φ1_qdec.
-    - apply Qdec_bot.
-  Qed.
+    Lemma φ1'_bounded : bounded 2 φ1'.
+    Proof.
+      unfold φ1'. rewrite pless_eq.
+      repeat solve_bounds.
+      - assumption.
+      - eapply subst_bound; first eassumption.
+        intros [|[|n]] H; cbn; solve_bounds.
+    Qed.
+    Lemma φ2'_bounded : bounded 2 φ2'.
+    Proof.
+      unfold φ2'. rewrite pless_eq.
+      repeat solve_bounds.
+      - assumption.
+      - eapply subst_bound; first eassumption.
+        intros [|[|n]] H; cbn; solve_bounds.
+    Qed.
+    Lemma φ1'_qdec : Qdec φ1'.
+    Proof.
+      apply Qdec_and; first assumption.
+      apply (@Qdec_bounded_forall _ 1).
+      apply Qdec_impl.
+      - apply Qdec_subst, φ2_qdec.
+      - apply Qdec_bot.
+    Qed.
+    Lemma φ2'_qdec : Qdec φ2'.
+    Proof.
+      apply Qdec_and; first assumption.
+      apply (@Qdec_bounded_forall _ 1).
+      apply Qdec_impl.
+      - apply Qdec_subst, φ1_qdec.
+      - apply Qdec_bot.
+    Qed.
 
-  Local Lemma DR1 x : P1 x -> Qeq ⊢ ∃ φ1'[(num x)..].
-  Proof.
-    intros HP1. eapply Σ1_completeness with (ρ := fun _ => 0).
-    { constructor. apply Σ1_subst. constructor. apply φ1'_qdec. }
-    { constructor. eapply subst_bound; first apply φ1'_bounded.
-      intros [|[|n]] H; try solve_bounds. apply num_bound. }
-    pose proof HP1 as H. erewrite (φ1_sem _ _) in H.
-    destruct H as [k Hk]. exists k.
-    split; first eassumption.
-    cbn. intros k' _ Hk'. apply (@P_disjoint x).
-    - eapply φ1_sem. exists k. apply Hk.
-    - eapply φ2_sem with (ρ := k .: (fun _ => 0)). exists k'.
-      rewrite subst_comp in Hk'.
-      erewrite bounded_subst. 1-2: eassumption.
-      intros [|[|n]] H; cbn.
-      + now rewrite num_subst.
-      + easy.
-      + lia.
-  Qed.
-  Local Lemma DR1' x : P2 x -> Qeq ⊢ ∃ φ2'[(num x)..].
-  Proof. 
-    intros HP1. eapply Σ1_completeness with (ρ := fun _ => 0).
-    { constructor. apply Σ1_subst. constructor. apply φ2'_qdec. }
-    { constructor. eapply subst_bound; first apply φ2'_bounded.
-      intros [|[|n]] H; try solve_bounds. apply num_bound. }
-    pose proof HP1 as H. erewrite (φ2_sem _ _) in H.
-    destruct H as [k Hk]. exists k.
-    split; first eassumption.
-    cbn. intros k' _ Hk'. apply (@P_disjoint x).
-    - eapply φ1_sem with (ρ := k .: (fun _ => 0)). exists k'.
-      rewrite subst_comp in Hk'.
-      erewrite bounded_subst. 1-2: eassumption.
-      intros [|[|n]] H; cbn.
-      + now rewrite num_subst.
-      + easy.
-      + lia.
-    - eapply φ2_sem. exists k. apply Hk.
-  Qed.
-  Local Lemma DR2 x : P2 x -> Qeq ⊢ ¬∃ φ1'[(num x)..].
-  Proof. 
-    cbn. intros HP2. 
-    assert (exists k, Qeq ⊢ φ2'[(num x)..][(num k)..]) as [k Hk].
-    { apply Σ1_witness.
-      - constructor. apply Qdec_subst. apply φ2'_qdec.
-      - eapply subst_bound; first apply φ2'_bounded.
-        intros [|[|n]] H; try solve_bounds. apply num_bound.
-      - apply Σ1_completeness with (ρ := id).
-        + constructor. apply Σ1_subst. constructor. apply φ2'_qdec.
-        + constructor. eapply subst_bound; first apply φ2'_bounded.
+    Local Lemma DR1 x : P1 x -> Qeq ⊢ ∃ φ1'[(num x)..].
+    Proof.
+      intros HP1. eapply Σ1_completeness with (ρ := fun _ => 0).
+      { constructor. apply Σ1_subst. constructor. apply φ1'_qdec. }
+      { constructor. eapply subst_bound; first apply φ1'_bounded.
+        intros [|[|n]] H; try solve_bounds. apply num_bound. }
+      pose proof HP1 as H. erewrite (φ1_sem _ _) in H.
+      destruct H as [k Hk]. exists k.
+      split; first eassumption.
+      cbn. intros k' _ Hk'. apply (@P_disjoint x).
+      - eapply φ1_sem. exists k. apply Hk.
+      - eapply φ2_sem with (ρ := k .: (fun _ => 0)). exists k'.
+        rewrite subst_comp in Hk'.
+        erewrite bounded_subst. 1-2: eassumption.
+        intros [|[|n]] H; cbn.
+        + now rewrite num_subst.
+        + easy.
+        + lia.
+    Qed.
+    Local Lemma DR1' x : P2 x -> Qeq ⊢ ∃ φ2'[(num x)..].
+    Proof. 
+      intros HP1. eapply Σ1_completeness with (ρ := fun _ => 0).
+      { constructor. apply Σ1_subst. constructor. apply φ2'_qdec. }
+      { constructor. eapply subst_bound; first apply φ2'_bounded.
+        intros [|[|n]] H; try solve_bounds. apply num_bound. }
+      pose proof HP1 as H. erewrite (φ2_sem _ _) in H.
+      destruct H as [k Hk]. exists k.
+      split; first eassumption.
+      cbn. intros k' _ Hk'. apply (@P_disjoint x).
+      - eapply φ1_sem with (ρ := k .: (fun _ => 0)). exists k'.
+        rewrite subst_comp in Hk'.
+        erewrite bounded_subst. 1-2: eassumption.
+        intros [|[|n]] H; cbn.
+        + now rewrite num_subst.
+        + easy.
+        + lia.
+      - eapply φ2_sem. exists k. apply Hk.
+    Qed.
+    Local Lemma DR2 x : P2 x -> Qeq ⊢ ¬∃ φ1'[(num x)..].
+    Proof. 
+      cbn. intros HP2. 
+      assert (exists k, Qeq ⊢ φ2'[(num x)..][(num k)..]) as [k Hk].
+      { apply Σ1_witness.
+        - constructor. apply Qdec_subst. apply φ2'_qdec.
+        - eapply subst_bound; first apply φ2'_bounded.
           intros [|[|n]] H; try solve_bounds. apply num_bound.
-        + apply DR1', soundness in HP2. apply HP2.
-          apply nat_is_Q_model. }
-    cbn in Hk. 
+        - apply Σ1_completeness with (ρ := id).
+          + constructor. apply Σ1_subst. constructor. apply φ2'_qdec.
+          + constructor. eapply subst_bound; first apply φ2'_bounded.
+            intros [|[|n]] H; try solve_bounds. apply num_bound.
+          + apply DR1', soundness in HP2. apply HP2.
+            apply nat_is_Q_model. }
+      cbn in Hk. 
 
-    custom_simpl. unfold "↑". fstart.
-    fintros "H". fdestruct "H". fdestruct "H".
+      custom_simpl. unfold "↑". fstart.
+      fintros "H". fdestruct "H". fdestruct "H".
 
-    pose proof (Qdec_le intu k). fspecialize (H x0). 
-    rewrite !pless_subst, !num_subst in H. cbn in H.
-    fdestruct H.
-    - fapply ("H0" (num k)).
-      + rewrite pless_subst. simpl_subst. ctx.
-      + simpl_subst. fassert (φ2[(num x)..][(num k)..]).
-        { fstop. eapply CE1, Weak; eauto. }
-        rewrite !subst_comp. erewrite bounded_subst.
-        * fapply "H2".
-        * eassumption.
-        * intros [|[|[|l]]]; cbn; (now rewrite ?num_subst + lia).
-    - rewrite !pless_subst in Hk.  cbn in Hk. rewrite num_subst in Hk.
-      fassert (∀ $0 ⧀= num k ~> ¬ φ1[$1 .: $0..][up (num x)..][up (num k)..]).
-      { fstop. eapply CE2, Weak; eauto. }
-      fapply ("H2" x0).
-      + rewrite pless_subst. simpl_subst. fapply "H1".
-      + rewrite !subst_comp. pattern (φ1[(num x).. >> subst_term x0..]). erewrite bounded_subst.
-        * fapply "H".
-        * eassumption.
-        * intros [|[|[|l]]]; cbn; (now rewrite ?num_subst + lia).
-  Qed.
+      pose proof (Qdec_le intu k). fspecialize (H x0). 
+      rewrite !pless_subst, !num_subst in H. cbn in H.
+      fdestruct H.
+      - fapply ("H0" (num k)).
+        + rewrite pless_subst. simpl_subst. ctx.
+        + simpl_subst. fassert (φ2[(num x)..][(num k)..]).
+          { fstop. eapply CE1, Weak; eauto. }
+          rewrite !subst_comp. erewrite bounded_subst.
+          * fapply "H2".
+          * eassumption.
+          * intros [|[|[|l]]]; cbn; (now rewrite ?num_subst + lia).
+      - rewrite !pless_subst in Hk.  cbn in Hk. rewrite num_subst in Hk.
+        fassert (∀ $0 ⧀= num k ~> ¬ φ1[$1 .: $0..][up (num x)..][up (num k)..]).
+        { fstop. eapply CE2, Weak; eauto. }
+        fapply ("H2" x0).
+        + rewrite pless_subst. simpl_subst. fapply "H1".
+        + rewrite !subst_comp. pattern (φ1[(num x).. >> subst_term x0..]). erewrite bounded_subst.
+          * fapply "H".
+          * eassumption.
+          * intros [|[|[|l]]]; cbn; (now rewrite ?num_subst + lia).
+    Qed.
 
-  Lemma weak_strong : exists φ, Σ1 φ /\
-    (forall x, P1 x -> Qeq ⊢ φ[(num x)..]) /\
-    (forall x, P2 x -> Qeq ⊢ ¬φ[(num x)..]).
-  Proof.
-    exists (∃ φ1'[$1 .: $0 ..]). repeat apply conj.
-    { do 2 constructor. apply Qdec_subst, φ1'_qdec. }
-    - intros x H%DR1. 
-      replace ((_)[_]) with (∃ φ1'[(num x)..]); first assumption.
-      change (∃ _)[_] with (∃ φ1'[$1 .: $0 ..][up (num x)..]).
-      f_equal. rewrite subst_comp. eapply bounded_subst; first apply φ1'_bounded.
-      intros [|[|n]] Hn; cbn. 2-3:solve_bounds.
-      now rewrite num_subst.
-    - intros x H%DR2.
-      replace ((_)[_]) with (∃ φ1'[(num x)..]); first assumption.
-      change (∃ _)[_] with (∃ φ1'[$1 .: $0 ..][up (num x)..]).
-      f_equal. rewrite subst_comp. eapply bounded_subst; first apply φ1'_bounded.
-      intros [|[|n]] Hn; cbn. 2-3:solve_bounds.
-      now rewrite num_subst.
-  Qed.
+    Lemma weak_strong' : exists φ, Σ1 φ /\ bounded 1 φ /\
+      (forall x, P1 x -> Qeq ⊢ φ[(num x)..]) /\
+      (forall x, P2 x -> Qeq ⊢ ¬φ[(num x)..]).
+    Proof.
+      exists (∃ φ1'[$1 .: $0 ..]). repeat apply conj.
+      { do 2 constructor. apply Qdec_subst, φ1'_qdec. }
+      { constructor. eapply subst_bound; first apply φ1'_bounded.
+        intros [|[|n]]; solve_bounds. }
+      - intros x H%DR1. 
+        replace ((_)[_]) with (∃ φ1'[(num x)..]); first assumption.
+        change (∃ _)[_] with (∃ φ1'[$1 .: $0 ..][up (num x)..]).
+        f_equal. rewrite subst_comp. eapply bounded_subst; first apply φ1'_bounded.
+        intros [|[|n]] Hn; cbn. 2-3:solve_bounds.
+        now rewrite num_subst.
+      - intros x H%DR2.
+        replace ((_)[_]) with (∃ φ1'[(num x)..]); first assumption.
+        change (∃ _)[_] with (∃ φ1'[$1 .: $0 ..][up (num x)..]).
+        f_equal. rewrite subst_comp. eapply bounded_subst; first apply φ1'_bounded.
+        intros [|[|n]] Hn; cbn. 2-3:solve_bounds.
+        now rewrite num_subst.
+    Qed.
+  End value_disjoint'.
+  Check weak_strong'.
+
+  Section weak_strong.
+    Existing Instance intu.
+
+    Variable φ1 φ2 : form.
+    Hypothesis (φ1_bounded : bounded 1 φ1) (φ2_bounded : bounded 1 φ2).
+    Hypothesis (φ1_Σ : Σ1 φ1) (φ2_qdec : Σ1 φ2).
+    Hypothesis (φ1_syn : forall x, P1 x <-> Qeq ⊢ φ1[(num x) ..])
+               (φ2_syn : forall x, P2 x <-> Qeq ⊢ φ2[(num x) ..]).
+
+    Lemma iff_iff φ ψ : (Qeq ⊢ φ <~> ψ) -> Qeq ⊢ φ <-> Qeq ⊢ ψ.
+    Proof.
+      intros H. split; intros H'; fapply H; exact H'.
+    Qed.
+    Lemma weak_strong : exists φ, Σ1 φ /\ bounded 1 φ /\
+      (forall x, P1 x -> Qeq ⊢ φ[(num x)..]) /\
+      (forall x, P2 x -> Qeq ⊢ ¬φ[(num x)..]).
+    Proof.
+      destruct (@Σ1_compression _ φ1 1) as (ψ1 & HQ1 & Hb1 & Hψ1), (@Σ1_compression _ φ2 1) as (ψ2 & HQ2 & Hb2 & Hψ2).
+      all: try assumption.
+      apply weak_strong' with (φ1 := ψ1[$1.:$0..]) (φ2 := ψ2[$1.:$0..]).
+      { eapply subst_bound; first eassumption. intros [|[|n]]; solve_bounds. }
+      { eapply subst_bound; first eassumption. intros [|[|n]]; solve_bounds. }
+      { now apply Qdec_subst. }
+      { now apply Qdec_subst. }
+      - intros x. rewrite φ1_syn. 
+        apply iff_iff.
+        apply (subst_Weak ((num x)..)) in Hψ1.
+        change (map _ _) with Qeq in Hψ1.
+        cbn in Hψ1.
+        assert (ψ1[$1 .: $0 ..][(num x) ..] = ψ1[up (num x)..]) as ->; last assumption.
+        { rewrite subst_comp. eapply bounded_subst; first eassumption.
+          intros [|[|n]] Hn; cbn.
+          - reflexivity.
+          - now rewrite num_subst.
+          - lia. }
+      - intros x. rewrite φ2_syn. 
+        apply iff_iff.
+        apply (subst_Weak ((num x)..)) in Hψ2.
+        change (map _ _) with Qeq in Hψ2.
+        cbn in Hψ2.
+        assert (ψ2[$1 .: $0 ..][(num x) ..] = ψ2[up (num x)..]) as ->; last assumption.
+        { rewrite subst_comp. eapply bounded_subst; first eassumption.
+          intros [|[|n]] Hn; cbn.
+          - reflexivity.
+          - now rewrite num_subst.
+          - lia. }
+    Qed.
+
+  End weak_strong.
 
 
 End value_disjoint.
+
